Factor out precomputation of nat<->string conversions in dataflow
This time, do it without adding an extra field to the precomputed data.

Performance characteristics:
JSAE Before: Finished transaction in 16.315 secs (16.271u,0.019s)
JSAE After: Finished transaction in 2.434 secs (2.424u,0.011s)

JSON Before: Finished transaction in 1.726 secs (1.72u,0.008s)
JSON After: Finished transaction in 0.78 secs (0.78u,0.s)

JSON first refine Before: Finished transaction in 0.38 secs (0.379u,0.s)
JSON first refine After: Finished transaction in 0.767 secs (0.763u,0.s)

JSAE first refine Before: Finished transaction in 1.294 secs (1.292u,0.003s)
JSAE first refine After: Finished transaction in 2.506 secs (2.496u,0.008s)

After    | File Name                                                            | Before   || Change
-------------------------------------------------------------------------------------------------------
3m47.14s | Total                                                                | 3m29.36s || +0m17.78s
-------------------------------------------------------------------------------------------------------
2m21.52s | Parsers/Refinement/SharpenedJSON                                     | 2m07.86s || +0m13.66s
0m22.98s | Parsers/Refinement/PossibleTerminalsSets                             | 0m19.68s || +0m03.30s
0m10.45s | Parsers/Refinement/IndexedAndAtMostOneNonTerminalReflective          | 0m10.23s || +0m00.21s
0m07.43s | Parsers/Refinement/IndexedAndAtMostOneNonTerminalReflectiveOpt       | 0m07.37s || +0m00.05s
0m05.56s | Parsers/Refinement/DisjointRulesRev                                  | 0m05.19s || +0m00.36s
0m04.43s | Parsers/Refinement/DisjointRules                                     | 0m04.08s || +0m00.34s
0m04.18s | Parsers/ContextFreeGrammar/Fix/ProdAbstractInterpretationDefinitions | 0m04.18s || +0m00.00s
0m03.72s | Parsers/ContextFreeGrammar/Fix/FromAbstractInterpretation            | 0m03.62s || +0m00.10s
0m02.68s | Parsers/Refinement/EmptyLemmas                                       | 0m02.65s || +0m00.03s
0m02.58s | Parsers/Refinement/SharpenedJSComment                                | 0m02.58s || +0m00.00s
0m02.47s | Parsers/Refinement/SharpenedExpressionPlus                           | 0m02.58s || -0m00.10s
0m02.30s | Parsers/Refinement/SharpenedExpressionPlusParen                      | 0m02.52s || -0m00.22s
0m02.30s | Parsers/Refinement/FixedLengthLemmas                                 | 0m02.24s || +0m00.05s
0m02.25s | Parsers/Refinement/BinOpBrackets/BinOpRules                          | 0m02.30s || -0m00.04s
0m01.89s | Parsers/Refinement/SharpenedStringLiteral                            | 0m01.88s || +0m00.01s
0m01.88s | Parsers/Refinement/SharpenedExpressionPlusParenParseTree             | 0m01.91s || -0m00.03s
0m01.68s | Parsers/Refinement/SharpenedABStar                                   | 0m01.69s || -0m00.01s
0m01.43s | Parsers/Refinement/SharpenedExpressionParen                          | 0m01.48s || -0m00.05s
0m01.29s | Parsers/Refinement/DisjointLemmas                                    | 0m01.32s || -0m00.03s
0m01.24s | Parsers/Refinement/Tactics                                           | 0m01.20s || +0m00.04s
0m01.04s | Parsers/ContextFreeGrammar/Fix/FromAbstractInterpretationDefinitions | 0m00.85s || +0m00.19s
0m01.00s | Parsers/Refinement/SharpenedABStarParseTree                          | 0m00.99s || +0m00.01s
0m00.84s | Parsers/ExtrOcamlParsers                                             | 0m00.96s || -0m00.12s

src/Parsers/Refinement/FixedLengthLemmas.v
@@ -3,6 +3,7 @@ Require Import Coq.Lists.List Coq.Strings.String.
 Require Import Coq.omega.Omega.
 Require Import Fiat.Parsers.ContextFreeGrammar.Core.
 Require Import Fiat.Parsers.ContextFreeGrammar.PreNotations.
+Require Import Fiat.Parsers.ContextFreeGrammar.Precompute.
 Require Import Fiat.Parsers.StringLike.Properties.
 Require Import Fiat.Common.
 Require Import Fiat.Common.NatFacts.
@@ -154,18 +155,24 @@ Definition length_result := lattice_for nat.
 Coercion collapse_length_result (v : length_result) : option nat
   := Eval cbv [collapse_lattice_for] in collapse_lattice_for v.
 
+Local Hint Immediate compile_item_data_of_abstract_interpretation : typeclass_instances.
+
 Definition length_of_any {Char} (G : pregrammar' Char)
+           (compiled_productions : list (opt.productions state))
 : String.string -> length_result
-  := fun nt => lookup_state (fold_grammar G) (@of_nonterminal _ (@rdp_list_predata _ G) nt).
+  := fun nt => lookup_state (fold_grammar G compiled_productions) (opt.compile_nonterminal nt).
 
 Section has_only_terminals.
   Context {Char}
           {HSLM : StringLikeMin Char}
           {HSL : StringLike Char}
           {HSLP : StringLikeProperties Char}
-          (G : pregrammar' Char) {n}
+          (G : pregrammar' Char)
+          compiled_productions
+          (compiled_productions_correct : List.map opt.compile_productions (List.map snd (pregrammar_productions G)) = compiled_productions)
+          {n}
           nt
-          (H : length_of_any G nt = constant n)
+          (H : length_of_any G compiled_productions nt = constant n)
           (str : String).
 
   Lemma has_only_terminals_parse_of_item_length
@@ -173,7 +180,7 @@ Section has_only_terminals.
     : length str = n.
   Proof.
     unfold length_of_any in H.
-    apply fold_grammar_correct_item in p.
+    eapply fold_grammar_correct_item in p; [ | eassumption ].
     rewrite H in p.
     destruct p; intuition.
   Qed.
@@ -183,7 +190,7 @@ Section has_only_terminals.
     : length str = n.
   Proof.
     unfold length_of_any in H.
-    apply fold_grammar_correct in p.
+    eapply fold_grammar_correct in p; [ | eassumption ].
     rewrite H in p.
     destruct p; intuition.
   Qed.
